Adattamento parziale correttezza compilatore. Modifiche a corredo

MasterThesis/LOOP/Interpreter.lean
@@ -6,13 +6,16 @@ namespace LOOP
 
 open LOOP.Com
 
-def eval (P : Com) (σ : Store) : Store :=
-  match P with
-  | SKIP    => σ
-  | ZER x   => Store.update x 0 σ
-  | ASN x y => Store.update x (σ y) σ
-  | INC x   => Store.update x ((σ x) + 1) σ
-  | SEQ P Q => (eval Q) (eval P σ)
-  | FOR x P => (fun σ' => (eval P σ'))^[σ x] σ
+def eval (P : Com) (s : State) : State :=
+  match s with
+  | none   => none
+  | some σ =>
+    match P with
+    | SKIP    => some σ
+    | ZER x   => some ([x ↦ 0] σ)
+    | ASN x y => some ([x ↦ (σ y)] σ)
+    | INC x   => some ([x ↦ ((σ x) + 1)] σ)
+    | SEQ P Q => (eval Q) (eval P σ)
+    | FOR x P => (fun σ' => (eval P σ'))^[σ x] σ
 
 end LOOP
