MasterThesis/Compiler/Commons.lean
@@ -1,0 +1,9 @@
+import MasterThesis.LOOP.Language
+import MasterThesis.SCORE.Language
+
+def eq_states (s : LOOP.State) (t : SCORE.State) : Prop :=
+  match s, t with
+  | some σ, some τ => ∀ (x : Ident), some ↑(σ x) = (τ x).head?
+  | _     , _      => False
+
+infix:50 "=ₛ" => eq_states
