MasterThesis/Compiler/Compiler_v1.lean
@@ -1,0 +1,22 @@
+import MasterThesis.SCORE.Language
+import MasterThesis.LOOP.Language
+
+namespace Compiler
+
+open LOOP Com
+open SCORE Com
+
+def l2s (Lc : LOOP.Com) : SCORE.Com :=
+  match Lc with
+  | .SKIP    => SKIP
+  | .ZER x   => CON x
+  | .ASN x y => if x ≠ y then
+                  CON x ;;
+                  FOR y (INC x)
+                else SKIP
+  | .INC x   => INC x
+  | .SEQ P Q => l2s P ;;
+                l2s Q
+  | .FOR x P => FOR x (l2s P)
+
+end Compiler
